compiler/src/compiler/FlatToRiscvFunctions.v
@@ -51,8 +51,9 @@ Section Proofs.
   Lemma stackalloc_words_nonneg: forall s,
       0 <= stackalloc_words s.
   Proof.
-    assert (bytes_per_word = 4 \/ bytes_per_word = 8). {
-      unfold bytes_per_word. destruct width_cases as [E | E]; rewrite E; cbv; auto.
+    clear h.
+    assert (Memory.bytes_per_word (bitwidth iset) = 4 \/ Memory.bytes_per_word (bitwidth iset) = 8). {
+      unfold Memory.bytes_per_word. destruct iset; cbv; auto.
     }
     induction s; simpl; Z.div_mod_to_equations; blia.
   Qed.
@@ -60,6 +61,7 @@ Section Proofs.
   Lemma framesize_nonneg: forall argvars resvars body,
       0 <= framelength (argvars, resvars, body).
   Proof.
+    clear h.
     intros. unfold framelength.
     pose proof (stackalloc_words_nonneg body).
     assert (bytes_per_word = 4 \/ bytes_per_word = 8). {
@@ -73,6 +75,7 @@ Section Proofs.
       fits_stack M N e s ->
       0 <= M /\ 0 <= N.
   Proof.
+    clear h.
     induction 1; try blia. pose proof (@framesize_nonneg argnames retnames body). blia.
   Qed.
 
@@ -96,7 +99,7 @@ Section Proofs.
       map.get impls f = Some impl ->
       iff1 (functions base rel_positions impls)
            (functions base rel_positions (map.remove impls f) *
-            program (word.add base (word.of_Z pos)) (compile_function rel_positions pos impl))%sep.
+            program iset (word.add base (word.of_Z pos)) (compile_function rel_positions pos impl))%sep.
   Proof.
     intros. unfold functions.
     match goal with
@@ -124,8 +127,8 @@ Section Proofs.
               | _ => fail 10000 P "is not a sep clause"
               end in
     lazymatch P with
-    | array ptsto_instr _ _ (compile_stmt _ _ _ ?Code) => Code
-    | ptsto_instr _ ?Instr => Instr
+    | array (ptsto_instr _) _ _ (compile_stmt _ _ _ ?Code) => Code
+    | ptsto_instr _ _ ?Instr => Instr
     | array ptsto_word _ _ ?Words => Words
     | functions _ _ ?E_Impl => E_Impl
     | _ => fail "no recognizable tag"
@@ -138,7 +141,7 @@ Section Proofs.
               end in
     lazymatch P with
     | array _ _ ?A _ => A
-    | ptsto_instr ?A _ => A
+    | ptsto_instr _ ?A _ => A
     | ptsto_word ?A _ => A
     | _ => fail "no recognizable address"
     end.
@@ -157,12 +160,12 @@ Section Proofs.
     | H: fits_stack _ _ _ ?Code |- fits_stack _ _ _ ?Code => exact H
     | H: map.get ?R RegisterNames.sp = Some _ |- map.get ?R RegisterNames.sp = Some _ => exact H
     | |- ?G => assert_fails (has_evar G);
-               solve [ simpl_addrs; solve_word_eq (@word_ok (@W (@def_params p)))
+               solve [ simpl_addrs; solve_word_eq (@word_ok (@W p))
                      | solve_stmt_not_too_big
                      | reflexivity
                      | assumption
                      | solve_divisibleBy4
-                     | solve_valid_machine (@word_ok (@W (@def_params p))) ]
+                     | solve_valid_machine (@word_ok (@W p)) ]
     | H: subset (footpr _) _ |- subset (footpr _) _ =>
       eapply rearrange_footpr_subset; [ exact H | solve [wwcancel] ]
     | |- _ => solve [wcancel_assumption]
@@ -205,9 +208,9 @@ Section Proofs.
     | |- exists (_: _), _ => eexists
     end;
     ssplit;
-    simpl_word_exprs (@word_ok (@W (@def_params p)));
+    simpl_word_exprs (@word_ok (@W p));
     match goal with
-    | |- _ => solve_word_eq (@word_ok (@W (@def_params p)))
+    | |- _ => solve_word_eq (@word_ok (@W p))
     | |- exists _, _ = _ /\ (_ * _)%sep _ =>
       eexists; split; cycle 1; [ wcancel_assumption | blia ]
     | |- _ => solve [rewrite ?of_list_list_union in *;
@@ -215,7 +218,7 @@ Section Proofs.
                         and slow everything down
                         change Z with Register in *; *)
                      map_solver (@locals_ok p h)]
-    | |- _ => solve [solve_valid_machine (@word_ok (@W (@def_params p)))]
+    | |- _ => solve [solve_valid_machine (@word_ok (@W p))]
     | |- _ => solve [eauto 3 using regs_initialized_put, preserve_valid_FlatImp_var_domain_put]
     | H: subset (footpr _) _ |- subset (footpr _) _ =>
       eapply rearrange_footpr_subset; [ exact H | solve [wwcancel] ]
@@ -226,7 +229,7 @@ Section Proofs.
     simpl_MetricRiscvMachine_get_set;
     simpl_g_get;
     rewrite ?@length_save_regs, ?@length_load_regs in *;
-    simpl_word_exprs (@word_ok (@W (@def_params p)));
+    simpl_word_exprs (@word_ok (@W p));
     repeat match goal with
            | |- _ /\ _ => split
            | |- exists _, _ => eexists
@@ -470,11 +473,14 @@ Section Proofs.
       | H: _ |- _ => let N := fresh in pose proof H as N;
                      apply map.getmany_of_list_length in N
       end.
+      assert (Memory.bytes_per_word (bitwidth iset) = bytes_per_word) as BPW. {
+        rewrite bitwidth_matches. reflexivity.
+      }
 
       (* put arguments on stack *)
       eapply runsTo_trans. {
         eapply save_regs_correct with (vars := args) (p_sp0 := p_sp)
-                (offset := (- bytes_per_word * Z.of_nat (List.length args))%Z); simpl; cycle -4.
+         (offset := (- Memory.bytes_per_word (bitwidth iset) * Z.of_nat (List.length args))%Z); simpl; cycle -4.
         - eapply rearrange_footpr_subset; [ eassumption | wwcancel ].
         - wcancel_assumption.
         - sidecondition.
@@ -647,7 +653,7 @@ Section Proofs.
     eapply runsTo_trans. {
       unfold good_e_impl, valid_FlatImp_fun in *. simp.
       eapply IHexec with (g := {|
-        p_sp := word.sub p_sp !(bytes_per_word * FL);
+        p_sp := word.sub p_sp !(Memory.bytes_per_word (bitwidth iset) * FL);
         e_pos := e_pos;
         e_impl := map.remove e_impl fname;
         program_base := program_base;
@@ -655,7 +661,7 @@ Section Proofs.
       simpl_MetricRiscvMachine_get_set;
       simpl_g_get;
       rewrite ?@length_save_regs, ?@length_load_regs in *;
-      simpl_word_exprs (@word_ok (@W (@def_params p)));
+      simpl_word_exprs (@word_ok (@W p));
       ssplit;
       subst FL.
       all: try safe_sidecond.
@@ -693,6 +699,7 @@ Section Proofs.
                | H: ?T |- _ => lazymatch T with
                                | map.putmany_of_list_zip _ _ _ = Some middle_regs0 => revert H
                                | assumptions => fail
+                               | _ = bytes_per_word => fail
                                | _ => clear H
                                end
                end.
@@ -842,7 +849,7 @@ Section Proofs.
 
     (* increase sp *)
     eapply runsToStep. {
-     eapply (run_Addi RegisterNames.sp RegisterNames.sp); try safe_sidecond.
+     eapply (run_Addi iset RegisterNames.sp RegisterNames.sp); try safe_sidecond.
      - simpl.
         rewrite map.get_put_diff by (clear; cbv; congruence).
         repeat match goal with
@@ -1121,6 +1128,7 @@ Section Proofs.
           rewrite map.get_put_same.
           f_equal.
           subst FL.
+          simpl_addrs.
           solve_word_eq word_ok. }
         {
           (* _ to 0 *)
@@ -1340,8 +1348,8 @@ Section Proofs.
       match goal with
       | H: map.putmany_of_list_zip _ _  (map.put (map.put _ _ _) _ ?v) = Some ?m2 |-
         map.get ?m2 _ = Some ?v' =>
-        rename H into D; clear -D h A;
-        replace v with v' in D by (solve_word_eq word_ok)
+        rename H into D; clear -D h A BPW;
+        replace v with v' in D by (simpl_addrs; solve_word_eq word_ok)
       end.
       eapply map.putmany_of_list_zip_get_oldval.
       * exact D.
@@ -1447,10 +1455,14 @@ Section Proofs.
       assert (bytes_per_word = 4 \/ bytes_per_word = 8) as B48. {
         unfold bytes_per_word. destruct width_cases as [E | E]; rewrite E; cbv; auto.
       }
+      assert (Memory.bytes_per_word (bitwidth iset) = bytes_per_word) as BPW. {
+        rewrite bitwidth_matches. reflexivity.
+      }
       assert (n / bytes_per_word <= Z.of_nat (List.length stack_trash)) as enough_stack_space. {
         match goal with
         | H: fits_stack _ _ _ _ |- _ => apply fits_stack_nonneg in H; move H at bottom
         end.
+        rewrite BPW in *.
         blia.
       }
       assert (0 <= n / bytes_per_word) as Nonneg. {
@@ -1480,7 +1492,7 @@ Section Proofs.
           rewrite Z.mul_opp_l.
           rewrite <- Z_div_exact_2.
           1: ring.
-          all: blia.
+          all: rewrite <- BPW; blia.
         }
         cbn [seps].
         reflexivity.
@@ -1501,7 +1513,7 @@ Section Proofs.
           simpl_MetricRiscvMachine_get_set;
           simpl_g_get;
           rewrite ?@length_save_regs, ?@length_load_regs in *;
-          simpl_word_exprs (@word_ok (@W (@def_params p)));
+          simpl_word_exprs (@word_ok (@W p));
           ssplit;
           cycle -5.
         { reflexivity. }
@@ -1525,16 +1537,17 @@ Section Proofs.
           | |- ?G => let t := type of Ab in replace G with t; [exact Ab|f_equal]
           end.
           rewrite length_flat_map with (n0 := Z.to_nat bytes_per_word).
-          - simpl_addrs. rewrite !Z2Nat.id by blia. rewrite <- Z_div_exact_2; blia.
+          - simpl_addrs. rewrite !Z2Nat.id by blia. rewrite <- BPW. rewrite <- Z_div_exact_2; blia.
           - clear. intros. rewrite HList.tuple.length_to_list. reflexivity.
         }
         { unfold map.split; split. 1: reflexivity. assumption. }
         { eassumption. }
         { eassumption. }
-        { match goal with
+        { rewrite BPW in *.
+          match goal with
           | H: fits_stack _ ?N _ _ |- fits_stack _ ?N' _ _ => replace N' with N; [exact H|blia]
           end. }
-        { f_equal. Z.div_mod_to_equations. blia. }
+        { f_equal. rewrite BPW in *. clear BPW. Z.div_mod_to_equations. blia. }
         { solve_stmt_not_too_big. }
         { eassumption. }
         { safe_sidecond. }
@@ -1545,7 +1558,7 @@ Section Proofs.
         { solve [eauto 3 using regs_initialized_put, preserve_valid_FlatImp_var_domain_put]. }
         { map_solver locals_ok. }
         { solve [eauto 3 using regs_initialized_put, preserve_valid_FlatImp_var_domain_put]. }
-      + intros. destruct_RiscvMachine middle. simp. subst. clear B48. run1done.
+      + intros. destruct_RiscvMachine middle. simp. subst. clear B48. rewrite BPW in *. clear BPW. run1done.
         * rewrite ?of_list_list_union in *.
           repeat match goal with
                  | H: (_ * _)%sep _ |- _ => clear H
