compiler/src/compiler/FlatToRiscvLiterals.v
@@ -82,9 +82,9 @@ Section FlatToRiscvLiterals.
       initialL.(getNextPc) = add initialL.(getPc) (word.of_Z 4) ->
       let insts := compile_lit x v in
       let d := mul (word.of_Z 4) (word.of_Z (Z.of_nat (List.length insts))) in
-      subset (footpr (program initialL.(getPc) insts * Rexec)%sep)
+      subset (footpr (program iset initialL.(getPc) insts * Rexec)%sep)
              (of_list initialL.(getXAddrs)) ->
-      (program initialL.(getPc) insts * Rexec * R)%sep initialL.(getMem) ->
+      (program iset initialL.(getPc) insts * Rexec * R)%sep initialL.(getMem) ->
       Primitives.valid_register x ->
       Primitives.valid_machine initialL ->
       runsTo (withRegs (map.put initialL.(getRegs) x (word.of_Z v))
@@ -106,6 +106,7 @@ Section FlatToRiscvLiterals.
       match_apply_runsTo.
       erewrite signExtend_nop; eauto; try blia.
     - (* TODO this step should be automatic *)
+      rewrite (@bitwidth_matches _ h) in *.
       assert (width = 32 \/ - 2 ^ 31 <= v < 2 ^ 31). {
         clear -E0 h.
         apply Bool.orb_true_iff in E0. destruct E0 as [E0 | E0].
@@ -116,6 +117,7 @@ Section FlatToRiscvLiterals.
       simpl in P.
       run1det. run1det.
       match_apply_runsTo.
+      rewrite E0.
       f_equal; [|solve_MetricLog].
       f_equal.
       + rewrite map.put_put_same. f_equal.
@@ -169,7 +171,9 @@ Section FlatToRiscvLiterals.
       run1det. repeat unfold_MetricLog.
       run1det. repeat unfold_MetricLog.
       match_apply_runsTo.
-      f_equal; [|simpl; solve_MetricLog].
+      rewrite (@bitwidth_matches _ h) in *.
+      rewrite E0.
+      f_equal; [|simpl; try solve_MetricLog].
       f_equal.
       + rewrite! map.put_put_same. f_equal. subst.
         apply word.unsigned_inj.
@@ -200,9 +204,9 @@ Section FlatToRiscvLiterals.
       initialL.(getNextPc) = add initialL.(getPc) (word.of_Z 4) ->
       let insts := compile_lit x v in
       let d := mul (word.of_Z 4) (word.of_Z (Z.of_nat (List.length insts))) in
-      subset (footpr (program initialL.(getPc) insts * Rexec)%sep)
+      subset (footpr (program iset initialL.(getPc) insts * Rexec)%sep)
              (of_list initialL.(getXAddrs)) ->
-      (program initialL.(getPc) insts * Rexec * R)%sep initialL.(getMem) ->
+      (program iset initialL.(getPc) insts * Rexec * R)%sep initialL.(getMem) ->
       valid_FlatImp_var x ->
       Primitives.valid_machine initialL ->
       runsTo (withRegs (map.put initialL.(getRegs) x (word.of_Z v))
